update engine certifications

core/SyntaxCertification.v
@@ -1,11 +1,17 @@
 Require Import core.Engine.
 Require Import core.Syntax.
+Require Import core.Semantics.
 Require Import core.TransformationConfiguration.
 Require Import core.Expressions.
 
 Section SyntaxCertification.
 
 Context {tc: TransformationConfiguration}.
+
+Definition evalOutputPatternLinkExpr_wrapper (sm: SourceModel) (sp: list SourceModelElement) (oe: TargetModelElement) (iter: nat)
+            (l: list TraceLink) (o: OutputPatternElement)
+  : option (list TargetModelLink) :=
+(evalOutputPatternLinkExpr sm sp oe (resolveIter l) iter o).
 
 Instance CoqTLSyntax :
   TransformationSyntax tc :=
@@ -30,7 +36,7 @@ Instance CoqTLSyntax :
       
       evalOutputPatternElementExpr := evalOutputPatternElementExpr;
       evalIteratorExpr := evalIteratorExpr;
-      evalOutputPatternLinkExpr := evalOutputPatternLinkExpr;
+      evalOutputPatternLinkExpr := evalOutputPatternLinkExpr_wrapper;
       evalGuardExpr := evalGuardExpr;
   }.
 
